ValueOpts.v
@@ -8,8 +8,11 @@ Require Import SetOperations Liveness Filter.
 Set Implicit Arguments.
 Unset Printing Records.
 
+Inductive eqn :=
+  | Eqn (o:nat) (e e':exp).
 
-Definition eqn := (exp * exp)%type.
+Definition EqnEq := 0.
+Definition EqnApx := 1.
 
 Inductive option_R (A B : Type) (eqA : A -> B -> Prop)
 : option A -> option B -> Prop :=
@@ -24,25 +27,86 @@ Instance option_R_sym A R `{Symmetric A R} : Symmetric (option_R R).
 hnf; intros ? [] []; eauto using option_R.
 Qed.
 
-Definition satisfies (E:onv val) (gamma:eqn) :=
-  option_eq eq (exp_eval E (fst gamma)) (exp_eval E (snd gamma)).
+Instance option_R_trans A R `{Transitive A R} : Transitive (option_R R).
+hnf; intros. inv H0; inv H1; econstructor; eauto.
+Qed.
 
-Inductive moreDef {X} : option X -> option X -> Prop :=
-  | moreDefSome v v' : moreDef (Some v) (Some v')
-  | moreDefNone x : moreDef None x.
+Inductive satisfies (E:onv val) : eqn -> Prop :=
+| SatisfiesEq e e'
+  : option_R eq (exp_eval E e) (exp_eval E e')
+    -> satisfies E (Eqn 0 e e')
+| SatisfiesApx e e'
+  : fstNoneOrR eq (exp_eval E e) (exp_eval E e')
+    -> satisfies E (Eqn 1 e e').
+
+Inductive eqnLt : eqn -> eqn -> Prop :=
+| EqnLtEq1 o o' e1 e1' e2 e2'
+  : _lt o o'
+    -> eqnLt (Eqn o e1 e2) (Eqn o' e1' e2')
+| EqnLtEq2 o e1 e1' e2 e2'
+  : expLt e1 e1'
+    -> eqnLt (Eqn o e1 e2) (Eqn o e1' e2')
+| EqnLtEq3 o e1 e2 e2'
+  : expLt e2 e2'
+    -> eqnLt (Eqn o e1 e2) (Eqn o e1 e2').
+
+Instance eqnLt_irr : Irreflexive eqnLt.
+hnf; intros; unfold complement.
+- induction x; inversion 1; subst; eauto;
+  try now eapply expLt_irr; eauto.
+  eapply StrictOrder_Irreflexive; eauto.
+Qed.
+
+Instance eqnLt_trans : Transitive eqnLt.
+hnf; intros.
+inv H; inv H0; eauto using eqnLt, expLt_trans.
+- econstructor. eapply StrictOrder_Transitive; eauto.
+Qed.
+
+Instance StrictOrder_eqnLt : OrderedType.StrictOrder eqnLt eq.
+econstructor.
+- eapply eqnLt_trans.
+- intros. intro. eapply eqnLt_irr. rewrite H0 in H.
+  eapply H.
+Qed.
+
+Notation "'Compare' x 'next' y" :=
+  (match x with
+    | Eq => y
+    | z => z
+  end) (at level 100).
+
+Fixpoint eqn_cmp (e e':eqn) :=
+  match e, e' with
+    | Eqn o e1 e2, Eqn o' e1' e2' =>
+      Compare _cmp o o' next
+      Compare _cmp e1 e1' next
+      Compare _cmp e2 e2' next Eq
+  end.
+
+Instance OrderedType_exp : OrderedType eqn :=
+ { _eq := eq;
+  _lt := eqnLt;
+  _cmp := eqn_cmp}.
+intros.
+destruct x,y; simpl eqn_cmp; try now (econstructor; eauto using eqnLt).
+pose proof (_compare_spec o o0); unfold _cmp in *; simpl in *.
+inv H; try now (econstructor; eauto using eqnLt).
+pose proof (_compare_spec e e0); unfold _cmp in *; simpl in *.
+inv H1; try now (econstructor; eauto using eqnLt).
+pose proof (_compare_spec e' e'0); unfold _cmp in *; simpl in *.
+inv H3; try now (econstructor; eauto 20 using eqnLt).
+Defined.
 
 Definition eqns := set eqn.
 
 Definition satisfiesAll (E:onv val) (Gamma:eqns) :=
   forall gamma, gamma ∈ Gamma -> satisfies E gamma.
 
-Definition sem_entails Gamma Γ' := forall E, satisfiesAll E Gamma -> satisfiesAll E Γ'.
-
-Definition freeVars (gamma:exp * exp) :=
-  let (e,e'):= gamma in Exp.freeVars e ∪ Exp.freeVars e'.
-
-Definition domain (gamma:exp * exp) :=
-  let (e,e'):= gamma in Exp.freeVars e.
+Definition freeVars (gamma:eqn) :=
+  match gamma with
+    | Eqn o e e' => Exp.freeVars e ∪ Exp.freeVars e'
+  end.
 
 Definition eqns_freeVars (Gamma:eqns) := fold union (map freeVars Gamma) ∅.
 
@@ -89,10 +153,12 @@ Definition moreDefinedArgs Gamma Y Y' :=
 Definition remove (Gamma:eqns) G :=
   filter (fun gamma => B[freeVars gamma ∩ G [=] ∅]) Gamma.
 
-Definition subst_eqn (ϱ : env exp) (e: eqn) :=
-  (subst_exp ϱ (fst e), subst_exp ϱ (snd e)).
+Definition subst_eqn (ϱ : env exp) (gamma: eqn) :=
+  match gamma with
+    | Eqn o e e' => Eqn o (subst_exp ϱ e) (subst_exp ϱ e')
+  end.
 
-Definition subst_eqns (ϱ : env exp) (G:eqns) :=
+Definition subst_eqns (ϱ : env exp) (G:eqns) : eqns :=
   map (subst_eqn ϱ) G.
 
 Definition sid := fun x => Var x.
@@ -107,15 +173,15 @@ Inductive eqn_sound : list (params*set var*eqns*eqns)
                       -> ann (list exp)
                       -> Prop :=
 | EqnOpr x Lv b e Gamma e' cl G G' ang
-  : eqn_sound Lv b ({{(Var x,e)}} ∪ {{(Var x,e')}} ∪ Gamma) ang cl
+  : eqn_sound Lv b ({{ Eqn EqnEq (Var x) e}} ∪ {{Eqn EqnEq (Var x) e'}} ∪ Gamma) ang cl
     (* make sure the rest conforms to the new assignment *)
     -> moreDefined Gamma e e'
     -> Exp.freeVars e' ⊆ G
     -> eqn_sound Lv (stmtExp x e b) Gamma
                 (ann1 (G,G') ang) (ann1 (e'::nil) cl)
 | EqnIf Lv e e' b1 b2 Gamma cl1 cl2 G G' ang1 ang2
-  : eqn_sound Lv b1 ({{(UnOp 0 e,Con val_true)}} ∪ Gamma) ang1 cl1
-  -> eqn_sound Lv b2 ({{(UnOp 0 e,Con val_false)}} ∪ Gamma) ang2 cl2
+  : eqn_sound Lv b1 ({{Eqn EqnEq (UnOp 0 e) (Con val_true)}} ∪ Gamma) ang1 cl1
+  -> eqn_sound Lv b2 ({{Eqn EqnEq (UnOp 0 e) (Con val_false)}} ∪ Gamma) ang2 cl2
   -> moreDefined Gamma e e'
   -> eqn_sound Lv (stmtIf e b1 b2) Gamma
               (ann2 (G,G') ang1 ang2) (ann2 (e'::nil) cl1 cl2)
@@ -249,7 +315,7 @@ Qed.
 Instance freeVars_Proper
   :  Proper (_eq ==> _eq) freeVars.
 Proof.
-  hnf; intros. inv H. inv H0. inv H1. reflexivity.
+  hnf; intros. inv H. reflexivity.
 Qed.
 
 Lemma eqns_freeVars_incl (Gamma:eqns) gamma
@@ -331,24 +397,64 @@ Lemma satisfiesAll_update_dead E Gamma Z vl
   -> satisfiesAll (E[Z <-- vl]) Gamma.
 Proof.
   intros. hnf; intros. hnf; intros.
-  hnf in H0; exploit H0; eauto. hnf in X.
-  erewrite exp_eval_agree; try eapply X.
-  symmetry.
-  erewrite exp_eval_agree; try eapply X.
-  symmetry.
-  erewrite <- minus_inane_set.
-  eapply update_with_list_agree_minus; eauto. reflexivity.
-  exploit eqns_freeVars_incl; eauto.
-  destruct gamma; simpl in *. rewrite <- H1.
-  revert H1 X0; clear_all; cset_tac; intuition; exfalso; eauto.
+  hnf in H0; exploit H0; eauto.
   inv X; eauto.
-  erewrite <- minus_inane_set.
-  symmetry.
-  eapply update_with_list_agree_minus; eauto. reflexivity.
-  exploit eqns_freeVars_incl; eauto.
-  destruct gamma; simpl in *. rewrite <- H1.
-  revert H1 X0; clear_all; cset_tac; intuition; exfalso; eauto.
-  inv X; eauto.
+  - inv H3. econstructor.
+    erewrite exp_eval_agree; try eapply H3.
+    symmetry.
+    erewrite exp_eval_agree; try eapply H3.
+    symmetry.
+    erewrite <- minus_inane_set.
+    eapply update_with_list_agree_minus; eauto. reflexivity.
+    exploit eqns_freeVars_incl; eauto.
+    rewrite <- H1.
+    simpl in X0.
+    revert H1 X0; clear_all; cset_tac; intuition; exfalso; eauto.
+    inv H3; eauto.
+    erewrite <- minus_inane_set.
+    symmetry.
+    eapply update_with_list_agree_minus; eauto. reflexivity.
+    exploit eqns_freeVars_incl; eauto.
+    rewrite <- H1.
+    revert H1 X0; simpl; clear_all; cset_tac; intuition; exfalso; eauto.
+    inv H3; eauto.
+  - inv H3.
+    + econstructor.
+      erewrite exp_eval_agree.
+      erewrite exp_eval_agree; try eapply H3.
+      symmetry.
+      erewrite <- minus_inane_set.
+      eapply update_with_list_agree_minus; eauto. reflexivity.
+      exploit eqns_freeVars_incl; eauto.
+      rewrite <- H1.
+      simpl in X0.
+      revert H1 X0; clear_all; cset_tac; intuition; exfalso; eauto.
+      inv H3; eauto.
+      erewrite <- minus_inane_set.
+      symmetry.
+      eapply update_with_list_agree_minus; eauto. reflexivity.
+      exploit eqns_freeVars_incl; eauto.
+      rewrite <- H1.
+      revert H1 X0; simpl; clear_all; cset_tac; intuition; exfalso; eauto.
+      inv H3; eauto.
+    + econstructor.
+      erewrite exp_eval_agree.
+      erewrite exp_eval_agree; try eapply H3.
+      symmetry.
+      erewrite <- minus_inane_set.
+      eapply update_with_list_agree_minus; eauto. reflexivity.
+      exploit eqns_freeVars_incl; eauto.
+      rewrite <- H1.
+      simpl in X0.
+      revert H1 X0; clear_all; cset_tac; intuition; exfalso; eauto.
+      inv H3; eauto.
+      erewrite <- minus_inane_set.
+      symmetry.
+      eapply update_with_list_agree_minus; eauto. reflexivity.
+      exploit eqns_freeVars_incl; eauto.
+      rewrite <- H1.
+      revert H1 X0; simpl; clear_all; cset_tac; intuition; exfalso; eauto.
+      inv H3; eauto.
 Qed.
 
 Lemma eval_exp_subst E y Y Z e
@@ -513,26 +619,24 @@ Proof.
 Qed.
 
 Lemma entails_eqns_trans Gamma e e' e''
-: (e, e') ∈ Gamma
-  -> (e', e'') ∈ Gamma
-  -> entails Gamma {(e, e''); {}}.
+: Eqn EqnEq e e' ∈ Gamma
+  -> Eqn EqnEq e' e'' ∈ Gamma
+  -> entails Gamma {Eqn EqnEq e e''; {}}.
 Proof.
   intros. hnf; intros.
   hnf; intros. cset_tac. hnf; intros. rewrite H2.
   simpl. exploit (H1 _ H); eauto.
   exploit (H1 _ H0); eauto.
   simpl in *. inv X; inv X0.
-  - econstructor.
-  - exfalso. congruence.
-  - exfalso. congruence.
-  - econstructor. congruence.
+  - econstructor. etransitivity; eauto.
 Qed.
 
-Lemma entails_eqns_refl e Gamma
-: entails Gamma {{ (e, e) }}.
+
+Lemma entails_eqns_apx_refl e Gamma
+: entails Gamma {{ Eqn EqnApx e e }}.
 Proof.
   hnf; intros. hnf; intros. hnf; intros. cset_tac. rewrite H0.
-  simpl. reflexivity.
+  econstructor. simpl. reflexivity.
 Qed.
 
 
@@ -552,36 +656,61 @@ Proof.
     exfalso. rewrite H in H8. cset_tac; intuition.
   - hnf; intros. eapply Add_Equal in H1. rewrite H1 in H10.
     eapply add_iff in H10. destruct H10.
-    + invc H10.
+    + hnf in H10; subst.
       hnf in H5; simpl in *. subst.
-      specialize (H5 V H6 (subst_eqn (sid [Z <-- Y]) (c,d))). exploit H5.
+      specialize (H5 V H6 (subst_eqn (sid [Z <-- Y]) gamma)). exploit H5.
       eapply in_subst_eqns; eauto. rewrite H1. cset_tac; intuition.
-      hnf in X. simpl in X.
-      do 2 erewrite <- eval_exp_subst in X; eauto.
-      hnf. simpl.
-      erewrite exp_eval_agree; [| |reflexivity].
-      erewrite exp_eval_agree with (e:=d); [| |reflexivity].
-      eapply X.
-      eapply update_with_list_agree; eauto.
-      eapply agree_on_incl; eauto.
-      assert ((c, d) ∈ s'). rewrite H1.
-      cset_tac; intuition.
-      exploit eqns_freeVars_incl; eauto. simpl in *.
-      rewrite H3 in X0.
-      rewrite <- (minus_union_set _ _ _ H4); eauto.
-      rewrite <- X0. eapply incl_minus_lr; cset_tac; intuition.
-      rewrite map_length. simpl in *.
-      exploit omap_length; eauto. congruence.
-      eapply update_with_list_agree; eauto.
-      eapply agree_on_incl; eauto.
-      assert ((c, d) ∈ s'). rewrite H1.
-      cset_tac; intuition.
-      exploit eqns_freeVars_incl; eauto.
-      rewrite H3 in X0. simpl in X0.
-      rewrite <- (minus_union_set _ _ _ H4); eauto.
-      rewrite <- X0. eapply incl_minus_lr; cset_tac; intuition.
-      rewrite map_length. simpl in *.
-      exploit omap_length; eauto. congruence.
+      hnf in X. destruct gamma. simpl in *. inv X.
+      * do 2 erewrite <- eval_exp_subst in H11; eauto.
+        econstructor.
+        erewrite exp_eval_agree; [| |reflexivity].
+        erewrite exp_eval_agree with (e:=e'); [| |reflexivity].
+        eapply H11.
+        eapply update_with_list_agree; eauto.
+        eapply agree_on_incl; eauto.
+        assert (Eqn 0 e e' ∈ s'). rewrite H1.
+        cset_tac; intuition.
+        exploit eqns_freeVars_incl; eauto. simpl in *.
+        rewrite H3 in X0.
+        rewrite <- (minus_union_set _ _ _ H4); eauto.
+        rewrite <- X0. eapply incl_minus_lr; cset_tac; intuition.
+        rewrite map_length. simpl in *.
+        exploit omap_length; eauto. congruence.
+        eapply update_with_list_agree; eauto.
+        eapply agree_on_incl; eauto.
+        assert (Eqn 0 e e' ∈ s'). rewrite H1.
+        cset_tac; intuition.
+        exploit eqns_freeVars_incl; eauto.
+        rewrite H3 in X0. simpl in X0.
+        rewrite <- (minus_union_set _ _ _ H4); eauto.
+        rewrite <- X0. eapply incl_minus_lr; cset_tac; intuition.
+        rewrite map_length. simpl in *.
+        exploit omap_length; eauto. congruence.
+      * do 2 erewrite <- eval_exp_subst in H11; eauto.
+        econstructor.
+        erewrite exp_eval_agree; [| |reflexivity].
+        erewrite exp_eval_agree with (e:=e'); [| |reflexivity].
+        eapply H11.
+        eapply update_with_list_agree; eauto.
+        eapply agree_on_incl; eauto.
+        assert (Eqn 1 e e' ∈ s'). rewrite H1.
+        cset_tac; intuition.
+        exploit eqns_freeVars_incl; eauto. simpl in *.
+        rewrite H3 in X0.
+        rewrite <- (minus_union_set _ _ _ H4); eauto.
+        rewrite <- X0. eapply incl_minus_lr; cset_tac; intuition.
+        rewrite map_length. simpl in *.
+        exploit omap_length; eauto. congruence.
+        eapply update_with_list_agree; eauto.
+        eapply agree_on_incl; eauto.
+        assert (Eqn 1 e e' ∈ s'). rewrite H1.
+        cset_tac; intuition.
+        exploit eqns_freeVars_incl; eauto.
+        rewrite H3 in X0. simpl in X0.
+        rewrite <- (minus_union_set _ _ _ H4); eauto.
+        rewrite <- X0. eapply incl_minus_lr; cset_tac; intuition.
+        rewrite map_length. simpl in *.
+        exploit omap_length; eauto. congruence.
     + rewrite H1 in H5.
       eapply H; try eapply H7; eauto.
       rewrite <- H3. rewrite H1.
@@ -606,30 +735,41 @@ Lemma satisfiesAll_update x Gamma V e e' y
   -> satisfiesAll V Gamma
   -> ⎣y ⎦ = exp_eval V e
   -> ⎣y ⎦ = exp_eval V e'
-  -> satisfiesAll (V [x <- ⎣y ⎦]) ({{(Var x, e)}} ∪ {(Var x, e'); {}} ∪ Gamma).
+  -> satisfiesAll (V [x <- ⎣y ⎦]) ({{Eqn EqnEq (Var x) e}} ∪ {Eqn EqnEq (Var x) e'; {}} ∪ Gamma).
 Proof.
   intros. hnf; intros. cset_tac. destruct H5. destruct H5.
-  - hnf; intros. invc H5; simpl in * |- *; subst.
+  - invc H5; simpl in * |- *; subst. econstructor.
     + erewrite <- exp_eval_agree; eauto. instantiate (1:=V).
-      rewrite <- H3. simpl. lud.
+      rewrite <- H3. simpl. lud. econstructor; eauto.
       exfalso; eauto.
       eapply agree_on_update_dead; eauto. reflexivity.
-  - hnf; intros. invc H5; simpl in * |- *; subst.
+  - invc H5; simpl in * |- *; subst. econstructor.
     + erewrite <- exp_eval_agree; eauto. instantiate (1:=V).
-      rewrite <- H4. simpl. lud.
+      rewrite <- H4. simpl. lud. econstructor; eauto.
       exfalso; eauto.
       eapply agree_on_update_dead; eauto. reflexivity.
-  - hnf in H1. exploit H2; eauto. hnf in X.
-    hnf.
-    erewrite <- exp_eval_agree; eauto.
-    symmetry.
-    erewrite <- exp_eval_agree; eauto. symmetry. eapply X.
-    eapply agree_on_update_dead; try reflexivity.
-    intro. eapply H. eapply in_eqns_freeVars; eauto.
-    destruct gamma; simpl; cset_tac; intuition.
-    eapply agree_on_update_dead; try reflexivity.
-    intro. eapply H. eapply in_eqns_freeVars; eauto.
-    destruct gamma; simpl; cset_tac; intuition.
+  - hnf in H1. exploit H2; eauto. inv X.
+    + econstructor.
+      erewrite <- exp_eval_agree; eauto.
+      symmetry.
+      erewrite <- exp_eval_agree; eauto. symmetry. eapply H6.
+      eapply agree_on_update_dead; try reflexivity.
+      intro. eapply H. eapply in_eqns_freeVars; eauto.
+      simpl; cset_tac; intuition.
+      eapply agree_on_update_dead; try reflexivity.
+      intro. eapply H. eapply in_eqns_freeVars; eauto.
+      simpl; cset_tac; intuition.
+    + econstructor.
+      erewrite (@exp_eval_agree _ _ e0); eauto.
+      erewrite exp_eval_agree with (e:=e'0); eauto.
+      symmetry.
+      eapply agree_on_update_dead; try reflexivity.
+      intro. eapply H. eapply in_eqns_freeVars; eauto.
+      simpl; cset_tac; intuition.
+      symmetry.
+      eapply agree_on_update_dead; try reflexivity.
+      intro. eapply H. eapply in_eqns_freeVars; eauto.
+      simpl; cset_tac; intuition.
 Qed.
 
 
@@ -644,13 +784,17 @@ Proof.
       hnf; intros. lud. exfalso; eauto.
       eapply H. eapply in_eqns_freeVars; eauto. rewrite e; eauto.
     }
-    + destruct gamma; simpl in *.
-      erewrite <- exp_eval_agree; eauto. instantiate (1:=V).
-      symmetry.
-      erewrite <- exp_eval_agree; eauto. instantiate (1:=V).
-      symmetry; exploit (H0 _ H1); eauto.
-      eapply agree_on_incl; eauto. cset_tac; intuition.
-      eapply agree_on_incl; eauto. cset_tac; intuition.
+    + exploit (H0 _ H1); eauto. inv X.
+      * econstructor.
+        erewrite exp_eval_agree; eauto. instantiate (1:=V).
+        erewrite exp_eval_agree with (e:=e'); eauto.
+        symmetry. eapply agree_on_incl; eauto. simpl; cset_tac; intuition.
+        symmetry. eapply agree_on_incl; eauto. simpl; cset_tac; intuition.
+      * econstructor.
+        erewrite exp_eval_agree; eauto. instantiate (1:=V).
+        erewrite exp_eval_agree with (e:=e'); eauto.
+        symmetry. eapply agree_on_incl; eauto. simpl; cset_tac; intuition.
+        symmetry. eapply agree_on_incl; eauto. simpl; cset_tac; intuition.
 Qed.
 
 Lemma satisfiesAll_monotone E Gamma Γ'
@@ -899,8 +1043,8 @@ Proof.
       econstructor; eauto using eq_sym. reflexivity.
       left. eapply IHEQN1; try eapply H9; eauto.
       * eapply satisfiesAll_union; split; eauto.
-        hnf; intros. cset_tac. inv H4. inv H15; inv H16.
-        hnf. simpl. rewrite <- H0. unfold option_lift1. simpl.
+        hnf; intros. cset_tac. invc H4.
+        econstructor. simpl. rewrite <- H0. unfold option_lift1. simpl.
         unfold val2bool in H3. destruct y; try congruence.
         destruct if; try congruence. constructor. reflexivity.
       * eapply simL'_update; eauto.
@@ -925,8 +1069,8 @@ Proof.
         {
           left. eapply IHEQN2; try eapply H13; eauto.
           - eapply satisfiesAll_union; split; eauto.
-            hnf; intros. cset_tac. inv H4. inv H15; inv H16.
-            hnf. simpl. rewrite <- H0. unfold option_lift1. simpl.
+            hnf; intros. cset_tac. invc H4.
+            econstructor. simpl. rewrite <- H0. unfold option_lift1. simpl.
             unfold val2bool in H3. destruct y; try congruence.
             destruct if; try congruence. constructor. reflexivity.
           - eapply simL'_update; eauto.
